LeanLambdaLibMathlib/LambdaLib.lean
@@ -1,0 +1,1 @@
+import LambdaLib.Basic
