LeanLambdaLibMathlib/LambdaLib/qterm.lean
@@ -1,0 +1,93 @@
+import LambdaLib.term
+
+instance Term.equivalence : Equivalence equiv where
+  refl := by
+    intros t
+    exists t
+    apply And.intro
+    · apply closure.refl
+    · apply closure.refl
+  symm := by
+    intros a b e
+    rcases e with ⟨t, r1, r2⟩
+    exact ⟨t, r2, r1⟩
+  trans := by
+    intros a b c e1 e2
+    rcases e1 with ⟨t1, r1, r2⟩
+    rcases e2 with ⟨t2, r3, r4⟩
+    have ⟨t, r5, r6⟩ := confluence r2 r3
+    exact ⟨t, transitivity r1 r5, transitivity r4 r6⟩
+
+instance Term.setoid : Setoid Term where
+  r := equiv
+  iseqv := Term.equivalence
+
+def QTerm := Quotient Term.setoid
+
+#check Quotient.map
+
+-- def liftCsr {A} {B} {R : Relation A} {R' : Relation B} {x y : A} (f : A → B)
+--   (ctr : ∀ {x y}, R x y → R' (f x) (f y))
+--   : closure R x y → closure R' (f x) (f y) :=
+
+theorem liftClosureUnion (f : Term → Term)
+  (respectStep : ∀ {x y}, Step x y → Step (f x) (f y))
+  (respectEta : ∀ {x y}, StepEta x y → StepEta (f x) (f y))
+  : ∀{x y}, AllStep x y → AllStep (f x) (f y) := by
+  intros x y eq
+  refine (liftCsr f ?_ eq)
+  intros x y step
+  exact (liftUnion f respectStep respectEta step)
+
+theorem respectStepLemma (f : Term → Term)
+  (respectStep : ∀ {x y}, Step x y → Step (f x) (f y))
+  (respectEta : ∀ {x y}, StepEta x y → StepEta (f x) (f y))
+  : ∀⦃x y⦄, x ≈ y → f x ≈ f y := by
+  intros x y eq
+  rcases eq with ⟨t, ⟨l, r⟩⟩
+  have l' := liftClosureUnion f respectStep respectEta l
+  have r' := liftClosureUnion f respectStep respectEta r
+  exact ⟨f t, ⟨l', r'⟩⟩
+
+theorem respectClosureUnion2 (f : Term → Term → Term)
+  (respectStep1 : ∀ {y x x'}, Step x x' → Step (f x y) (f x' y))
+  (respectEta1 : ∀ {y x x'}, StepEta x x' → StepEta (f x y) (f x' y))
+  (respectStep2 : ∀ {x y y'}, Step y y' → Step (f x y) (f x y'))
+  (respectEta2 : ∀ {x y y'}, StepEta y y' → StepEta (f x y) (f x y'))
+  : ∀{x x' y y'}, AllStep x x' → AllStep y y' → AllStep (f x y) (f x' y') := by
+  intros x x' y y' eq
+  refine (liftCsr2 f ?_ ?_ eq)
+  · intros x x' y step
+    exact (liftUnion (fun x => f x y) respectStep1 respectEta1 step)
+  · intros x x' y step
+    exact (liftUnion (f x) respectStep2 respectEta2 step)
+
+theorem respectStepLemma2 (f : Term → Term → Term)
+  (respectStep1 : ∀ {y x x'}, Step x x' → Step (f x y) (f x' y))
+  (respectEta1 : ∀ {y x x'}, StepEta x x' → StepEta (f x y) (f x' y))
+  (respectStep2 : ∀ {x y y'}, Step y y' → Step (f x y) (f x y'))
+  (respectEta2 : ∀ {x y y'}, StepEta y y' → StepEta (f x y) (f x y'))
+  : ∀⦃x x'⦄, x ≈ x' → ∀⦃y y'⦄, y ≈ y' → f x y ≈ f x' y' := by
+  intros x x' eqx y y' eqy
+  rcases eqx with ⟨tx, ⟨lx, rx⟩⟩
+  rcases eqy with ⟨ty, ⟨ly, ry⟩⟩
+  have l' := respectClosureUnion2 f respectStep1 respectEta1 respectStep2 respectEta2 lx ly
+  have r' := respectClosureUnion2 f respectStep1 respectEta1 respectStep2 respectEta2 rx ry
+  exact ⟨f tx ty, ⟨l', r'⟩⟩
+
+def lam (s : String) (t : QTerm) : QTerm :=
+  Quotient.map (Term.lam s) (respectStepLemma (Term.lam s) Step.lam StepEta.lam) t
+
+def app (t1 t2 : QTerm) : QTerm :=
+  Quotient.map₂ Term.app
+    (respectStepLemma2 Term.app Step.app1 StepEta.app1 Step.app2 StepEta.app2) t1 t2
+
+def var (i : Nat) : QTerm := Quotient.mk _ (Term.var i)
+
+-- TODO: namespaces
+def lift2 (i : Nat) (t : QTerm) : QTerm :=
+  Quotient.map (lift i) (respectStepLemma (lift i) liftStep etaLift) t
+
+def subst2 (i : Nat) (t1 t2 : QTerm) : QTerm :=
+  Quotient.map₂ (subst i)
+    (respectStepLemma2 (subst i) _ _ (substStep _ _) (etaSubst2 _ _)) t1 t2
